Yoneda: minor cleanup realted to le_induction

theories/Cubical/Yoneda.v
@@ -118,37 +118,36 @@ Ltac invert_le Hpq :=
                    now apply le_contra in Hpq |]
   end.
 
-Theorem le_induction {n p} (Hpn : p <= n) (P: forall p (Hpn: p <= n), Type)
+Theorem le_induction {n p} (Hp : p <= n) (P: forall p (Hp: p <= n), Type)
   (H_base: P n (¹ n))
-  (H_step: forall p (Hpn: p.+1 <= n) (H: P p.+1 Hpn), P p (↓ Hpn)): P p Hpn.
+  (H_step: forall p (Hp: p.+1 <= n) (H: P p.+1 Hp), P p (↓ Hp)): P p Hp.
 Proof.
-  intros *. induction n.
-  pose (Q := leYoneda_implies_le Hpn); pose (R := Peano.le_0_n).
+  induction n. pose (Q := leYoneda_implies_le Hp); pose (R := Peano.le_0_n).
   assert (p = 0) as -> by lia; now exact H_base.
-  pose (Q := leYoneda_implies_le Hpn); apply le_lt_eq_dec in Q;
+  pose (Q := leYoneda_implies_le Hp); apply le_lt_eq_dec in Q;
   destruct Q. apply le_implies_leYoneda in l. apply (H_step p l).
-  refine (IHn (⇓ l) (fun p Hpn => P p.+1 (⇑ Hpn)) H_base _).
-  change (⇑ (↓ ?H)) with (↑ H); intros q Hqn; now exact (H_step q.+1 (⇑ Hqn)).
+  now exact (IHn (⇓ l) (fun p Hp => P p.+1 (⇑ Hp)) H_base
+    (fun q Hq => H_step q.+1 (⇑ Hq))).
   assert (p = n.+1) as -> by assumption. now exact H_base.
 Defined.
 
-Definition le_induction' {n p} (Hpn: p.+1 <= n.+1)
-  (P: forall p (Hpn: p.+1 <= n.+1), Type)
+Definition le_induction' {n p} (Hp: p.+1 <= n.+1)
+  (P: forall p (Hp: p.+1 <= n.+1), Type)
   (H_base: P n (¹ n.+1))
-  (H_step: forall p (H : p.+2 <= n.+1), P p.+1 H -> P p (↓ H)): P p Hpn :=
-  le_induction (⇓ Hpn) (fun p Hpn => P p (⇑ Hpn)) H_base
-    (fun q Hqn => H_step q (⇑ Hqn)).
+  (H_step: forall p (H : p.+2 <= n.+1), P p.+1 H -> P p (↓ H)): P p Hp :=
+  le_induction (⇓ Hp) (fun p Hp => P p (⇑ Hp)) H_base
+    (fun q Hq => H_step q (⇑ Hq)).
 
-Definition le_induction'' {n p} (Hpn : p.+2 <= n.+2)
-  (P : forall p (Hpn: p.+2 <= n.+2), Type)
+Definition le_induction'' {n p} (Hp : p.+2 <= n.+2)
+  (P : forall p (Hp: p.+2 <= n.+2), Type)
   (H_base: P n (¹ n.+2))
-  (H_step: forall p (H : p.+3 <= n.+2), P p.+1 H -> P p (↓ H)): P p Hpn :=
-  le_induction' (⇓ Hpn) (fun p Hpn => P p (⇑ Hpn)) H_base
-    (fun q Hqn => H_step q (⇑ Hqn)).
+  (H_step: forall p (H : p.+3 <= n.+2), P p.+1 H -> P p (↓ H)): P p Hp :=
+  le_induction' (⇓ Hp) (fun p Hp => P p (⇑ Hp)) H_base
+    (fun q Hq => H_step q (⇑ Hq)).
 
-Lemma le_induction_computes {n p P H_base H_step} {Hpn: p.+1 <= n}:
-  le_induction (↓ Hpn) P H_base H_step =
-    H_step p Hpn (le_induction Hpn P H_base H_step).
+Lemma le_induction_computes {n p P H_base H_step} {Hp: p.+1 <= n}:
+  le_induction (↓ Hp) P H_base H_step =
+    H_step p Hp (le_induction Hp P H_base H_step).
 Proof.
 Admitted.
 
@@ -157,8 +156,8 @@ Lemma le_induction'_base_computes {n P H_base H_step}:
 Proof.
 Admitted.
 
-Lemma le_induction'_step_computes {n p P H_base H_step} {Hpn: p.+2 <= n.+1}:
-  le_induction' (↓ Hpn) P H_base H_step =
-    H_step p Hpn (le_induction' Hpn P H_base H_step).
+Lemma le_induction'_step_computes {n p P H_base H_step} {Hp: p.+2 <= n.+1}:
+  le_induction' (↓ Hp) P H_base H_step =
+    H_step p Hp (le_induction' Hp P H_base H_step).
 Proof.
 Admitted.
